\documentclass{article}
\usepackage[margin=0.78in]{geometry}
\usepackage{fancyhdr}
\usepackage{amsmath}
\usepackage{enumerate}

\usepackage{hyperref} % USE THIS LINE FOR SOLUTION LINKS
%\newcommand{\href}[2]{#2} % USE THIS LINE TO SUPPRESS SOLUTION LINKS

\fancyhf{}
\lhead{Series Strategy Problems List -- Dr. Edward D. Kim (University of Wisconsin - La Crosse)}
\fancyfoot[C]{}

\begin{document}
\pagestyle{fancy}

\noindent
First go through the book and write down each of the series tests. (Be sure to clearly write the {\bf requirements} for using each test. Some of the tests will immediately require you to study a sequence.) Compare and contrast: Take one row at a time. After completing a row, reflect on what test/strategy was needed for each series. Then make up an example which can be solved using the same test. In each case, determine if the series diverges, converges absolutely, or converges conditionally.

\begin{enumerate}[(a)]

\item\quad
\href{https://edward-kim-math.github.io/key/series/a1.pdf}{Does the infinite sequence $\displaystyle a_n = \frac1n$ converge?
Does the infinite series $\displaystyle \sum_{n=1}^\infty \frac1n$ converge?}

\vfill

\item \quad 
\href{https://edward-kim-math.github.io/key/series/b1.pdf}{$\displaystyle \sum_{n=1}^\infty \frac1n$} %b1
\quad
\href{https://edward-kim-math.github.io/key/series/b2.pdf}{$\displaystyle \sum_{n=1}^\infty \frac{(-1)^n}n$} %b2
\quad
\href{https://edward-kim-math.github.io/key/series/b3.pdf}{$\displaystyle \sum_{n=1}^\infty \frac{(-1)^n}{n^2}$} %b3
\quad
\href{https://edward-kim-math.github.io/key/series/b4.pdf}{$\displaystyle \sum_{n=1}^\infty \frac1{n^{0.9}}$} %b4
\quad
\href{https://edward-kim-math.github.io/key/series/b5.pdf}{$\displaystyle \sum_{n=1}^\infty \frac1{0.9^n}$}
\quad
\href{https://edward-kim-math.github.io/key/series/b6.pdf}{$\displaystyle \sum_{n=1}^\infty \frac1{n^2}$}
\quad
\href{https://edward-kim-math.github.io/key/series/b7.pdf}{$\displaystyle \sum_{n=1}^\infty \frac1{2^n}$}
\quad
\href{https://edward-kim-math.github.io/key/series/b8.pdf}{$\displaystyle \sum_{n=1}^\infty n^2$}
\quad
\href{https://edward-kim-math.github.io/key/series/b9.pdf}{$\displaystyle \sum_{n=1}^\infty 2^n$}

\vfill

\item\quad
%$\displaystyle\sum_{n=1}^\infty \frac{1}{2^n}$
%\quad
%$\displaystyle\sum_{n=1}^\infty 2^n$
%\quad
\href{https://edward-kim-math.github.io/key/series/c1.pdf}{$\displaystyle\sum_{n=1}^\infty \frac{3}{2^n}$}
\quad
\href{https://edward-kim-math.github.io/key/series/c2.pdf}{$\displaystyle\sum_{n=1}^\infty \frac{3^n}{2^n}$}
\quad
\href{https://edward-kim-math.github.io/key/series/c3.pdf}{$\displaystyle\sum_{n=1}^\infty \frac{2^n}{3^n}$}
\quad
\href{https://edward-kim-math.github.io/key/series/c4.pdf}{$\displaystyle\sum_{n=1}^\infty \frac{e^e}{2^n}$}
\quad
\href{https://edward-kim-math.github.io/key/series/c5.pdf}{$\displaystyle\sum_{n=1}^\infty \frac{e^n}{2^n}$}
\quad
\href{https://edward-kim-math.github.io/key/series/c6.pdf}{$\displaystyle\sum_{n=1}^\infty \frac{n^e}{2^n}$}
\quad
\href{https://edward-kim-math.github.io/key/series/c7.pdf}{$\displaystyle\sum_{n=1}^\infty \frac{e^n}{n^2}$}
\quad
\href{https://edward-kim-math.github.io/key/series/c8.pdf}{$\displaystyle\sum_{n=1}^\infty \frac{n^e}{n^2}$}
\quad

\vfill



\item \quad 
\href{https://edward-kim-math.github.io/key/series/d1.pdf}{$\displaystyle \sum_{n=1}^\infty \textstyle \left(\frac1n\right)^n$}
\quad
\href{https://edward-kim-math.github.io/key/series/d2.pdf}{$\displaystyle \sum_{n=1}^\infty \textstyle \left(1+\frac1n\right)^n$}
\quad
\href{https://edward-kim-math.github.io/key/series/d3.pdf}{$\displaystyle \sum_{n=1}^\infty \textstyle \left(\frac89+\frac1n\right)^n$}
\quad
\href{https://edward-kim-math.github.io/key/series/d4.pdf}{$\displaystyle \sum_{n=1}^\infty \left(\frac{8n+1}{9n-1}+\frac1n\right)^n$}
\quad
\href{https://edward-kim-math.github.io/key/series/d5.pdf}{$\displaystyle \sum_{n=1}^\infty \left(\frac{\ln n}{9n-1}\right)^n$}
\quad
\href{https://edward-kim-math.github.io/key/series/d6.pdf}{$\displaystyle \sum_{n=1}^\infty \left(\frac{\sin n}{9n-1}\right)^n$}

\vfill

\item \quad 
\href{https://edward-kim-math.github.io/key/series/e1.pdf}{$\displaystyle \sum_{n=2}^\infty \frac{\ln n}{n}$}
\quad
\href{https://edward-kim-math.github.io/key/series/e2.pdf}{$\displaystyle \sum_{n=2}^\infty \frac1{n \ln n}$}
\quad
\href{https://edward-kim-math.github.io/key/series/e3.pdf}{$\displaystyle \sum_{n=2}^\infty \frac1{n (\ln n)^{100}}$}
\quad
%$\displaystyle \sum_{n=2}^\infty \left(\frac1{n \ln n} - \frac1{(n+1) \ln (n+1)}\right)$
%\quad
\href{https://edward-kim-math.github.io/key/series/e4.pdf}{$\displaystyle \sum_{n=2}^\infty \left(\frac1{\ln n} - \frac1{\ln (n+1)}\right)$}
\quad
\href{https://edward-kim-math.github.io/key/series/e5.pdf}{$\displaystyle \sum_{n=1}^\infty n^7e^{-n^8}$}

\vfill

\item \quad 
\href{https://edward-kim-math.github.io/key/series/f1.pdf}{$\displaystyle \sum_{n=1}^\infty \frac1{n(n+1)}$}
\quad
\href{https://edward-kim-math.github.io/key/series/f2.pdf}{$\displaystyle \sum_{n=1}^\infty \frac1{n(n+2)}$}
%\quad
%$\displaystyle \sum_{n=1}^\infty \frac1{n(n+3)}$
%\quad
%$\displaystyle \sum_{n=2}^\infty \frac1{n(n-1)}$

\vfill

\item \quad 
\href{https://edward-kim-math.github.io/key/series/g1.pdf}{$\displaystyle \sum_{n=2}^\infty \frac1{n^2-1}$}
\quad
\href{https://edward-kim-math.github.io/key/series/g2.pdf}{$\displaystyle \sum_{n=2}^\infty \frac{2n}{n^2-1}$}
\quad
\href{https://edward-kim-math.github.io/key/series/g3.pdf}{$\displaystyle \sum_{n=2}^\infty \frac{n+2}{n^2-1}$}
\quad
\href{https://edward-kim-math.github.io/key/series/g4.pdf}{$\displaystyle \sum_{n=2}^\infty \frac{n}{n^3-1}$}
\quad
\href{https://edward-kim-math.github.io/key/series/g5.pdf}{$\displaystyle \sum_{n=2}^\infty \frac{n+2}{n^3-1}$}
\quad
\href{https://edward-kim-math.github.io/key/series/g6.pdf}{$\displaystyle \sum_{n=2}^\infty \frac{n^2+2}{n^3-1}$}
\vfill

\item \quad 
\href{https://edward-kim-math.github.io/key/series/h1.pdf}{$\displaystyle \sum_{n=2}^\infty \frac1{n^2+1}$}
\quad
\href{https://edward-kim-math.github.io/key/series/h2.pdf}{$\displaystyle \sum_{n=2}^\infty \frac{2n}{n^2+1}$}
\quad
\href{https://edward-kim-math.github.io/key/series/h3.pdf}{$\displaystyle \sum_{n=2}^\infty \frac{n+2}{n^2+1}$}
\quad
\href{https://edward-kim-math.github.io/key/series/h4.pdf}{$\displaystyle \sum_{n=2}^\infty \frac{n}{n^3+1}$}
\quad
\href{https://edward-kim-math.github.io/key/series/h5.pdf}{$\displaystyle \sum_{n=2}^\infty \frac{n+2}{n^3+1}$}
\quad
\href{https://edward-kim-math.github.io/key/series/h6.pdf}{$\displaystyle \sum_{n=2}^\infty \frac{n^2+2}{n^3+1}$}
\quad
\href{https://edward-kim-math.github.io/key/series/h7.pdf}{$\displaystyle \sum_{n=2}^\infty \frac{\arctan n}{n^2+1}$}
\vfill

\item \quad 
\href{https://edward-kim-math.github.io/key/series/i1.pdf}{$\displaystyle \sum_{n=1}^\infty \frac1{3n-1}$}
\quad
\href{https://edward-kim-math.github.io/key/series/i2.pdf}{$\displaystyle \sum_{n=1}^\infty \frac1{3n^5+n^4+n^3+n^2+n+1}$}
\quad
\href{https://edward-kim-math.github.io/key/series/i3.pdf}{$\displaystyle \sum_{n=1}^\infty \frac{15n^4 + 4n^3 + 3n^2+2n + 1}{3n^5+n^4+n^3+n^2+n+1}$}

\vfill

\item \quad 
\href{https://edward-kim-math.github.io/key/series/j1.pdf}{$\displaystyle \sum_{n=1}^\infty \frac1{5^n+1}$}
\quad
\href{https://edward-kim-math.github.io/key/series/j2.pdf}{$\displaystyle \sum_{n=1}^\infty \frac1{5^n-1}$}
\quad
\href{https://edward-kim-math.github.io/key/series/j3.pdf}{$\displaystyle \sum_{n=1}^\infty \frac{5^n \ln 5}{5^n-1}$}


\vfill

\item \quad 
\href{https://edward-kim-math.github.io/key/series/k1.pdf}{$\displaystyle \sum_{n=1}^\infty \frac{2+\cos \pi n}n$}
\quad
\href{https://edward-kim-math.github.io/key/series/k2.pdf}{$\displaystyle \sum_{n=1}^\infty \frac{\cos \pi n}n$}
\quad
\href{https://edward-kim-math.github.io/key/series/k3.pdf}{$\displaystyle \sum_{n=1}^\infty \frac{\cos \pi n}{n^2}$}
\quad
\href{https://edward-kim-math.github.io/key/series/k4.pdf}{$\displaystyle \sum_{n=1}^\infty \frac{\cos \frac\pi3 n}{n^2}$}
\quad
\href{https://edward-kim-math.github.io/key/series/k5.pdf}{$\displaystyle \sum_{n=1}^\infty \frac{2n+\cos n}{n^2 + \sin n}$}
\quad
\href{https://edward-kim-math.github.io/key/series/k6.pdf}{$\displaystyle \sum_{n=1}^\infty \left(\frac{2\pi+\cos n}n\right)^n$}

\vfill

\item \quad 
\href{https://edward-kim-math.github.io/key/series/l1.pdf}{$\displaystyle \sum_{n=1}^\infty \frac{(-1)^n}{n+1}$}
\quad
\href{https://edward-kim-math.github.io/key/series/l2.pdf}{$\displaystyle \sum_{n=1}^\infty \frac{(-1)^n n}{n+1}$}
\quad
\href{https://edward-kim-math.github.io/key/series/l3.pdf}{$\displaystyle \sum_{n=1}^\infty \frac{1}{(n+1)^n}$}

\vfill

\item \quad 
\href{https://edward-kim-math.github.io/key/series/m1.pdf}{$\displaystyle\sum_{n=1}^\infty \frac{1}{n!}$}
\quad
\href{https://edward-kim-math.github.io/key/series/m2.pdf}{$\displaystyle\sum_{n=1}^\infty \frac{n^n}{n!}$}
\quad
\href{https://edward-kim-math.github.io/key/series/m3.pdf}{$\displaystyle\sum_{n=1}^\infty \frac{n!}{n^n}$}
\quad
\href{https://edward-kim-math.github.io/key/series/m4.pdf}{$\displaystyle \sum_{n=1}^\infty n!$}
\quad
\href{https://edward-kim-math.github.io/key/series/m5.pdf}{$\displaystyle \sum_{n=1}^\infty \frac{n}{n!}$}
\quad
\href{https://edward-kim-math.github.io/key/series/m6.pdf}{$\displaystyle \sum_{n=1}^\infty \frac{2^n}{n!}$}
\quad
\href{https://edward-kim-math.github.io/key/series/m7.pdf}{$\displaystyle \sum_{n=1}^\infty \frac{2^n}{n^2}$}
\quad
\href{https://edward-kim-math.github.io/key/series/m8.pdf}{$\displaystyle \sum_{n=1}^\infty \frac{n^2}{2^n}$}
\quad
\href{https://edward-kim-math.github.io/key/series/m9.pdf}{$\displaystyle \sum_{n=1}^\infty \frac{n!}{(2n)!}$}
\quad

\vfill


\item\quad
\href{https://edward-kim-math.github.io/key/series/n1.pdf}{$\displaystyle\sum_{n=1}^\infty \frac{1}{n^{3/2}}$}
\quad
\href{https://edward-kim-math.github.io/key/series/n2.pdf}{$\displaystyle\sum_{n=1}^\infty \frac{1}{n^{2/3}}$}
\quad
\href{https://edward-kim-math.github.io/key/series/n3.pdf}{$\displaystyle\sum_{n=1}^\infty \frac{n^2 + 1}{n^3+7}$}
\quad
\href{https://edward-kim-math.github.io/key/series/n4.pdf}{$\displaystyle\sum_{n=1}^\infty \frac{n^2 + 1}{n^4+7}$}
\quad
\href{https://edward-kim-math.github.io/key/series/n5.pdf}{$\displaystyle\sum_{n=1}^\infty \frac{n^2 - 1}{n^3+7}$}
\quad
\href{https://edward-kim-math.github.io/key/series/n6.pdf}{$\displaystyle\sum_{n=1}^\infty \frac{n^2 - 1}{n^4+7}$}
\quad

\end{enumerate}

\newpage

\noindent
Techniques for series:
\begin{itemize}
\item If you can find the limit of $s_n$, the sequence of partial sums, do this, because this is the value of the series.
\begin{itemize}
\item Sometimes, finding the limit of $s_n$ is done after cancellations in a telescoping series.
\item Sometimes, finding the limit of $s_n$ is done after partial fractions leads to cancellations in a telescoping series.
\end{itemize}
\item Test for Divergence
\item Geometric Series Test
\item Integral Test
\item $p$-series Test
\item (Direct) Comparison Test
\item Limit Comparison Test
\item Alternating Series Test
\item Absolute Convergence Test
\item Ratio Test
\item Root Test
\end{itemize}

\end{document}

\vfill

\item \quad 
$\displaystyle \sum_{n=1}^\infty $
\quad
$\displaystyle \sum_{n=1}^\infty $
\quad
$\displaystyle \sum_{n=1}^\infty $
\quad
$\displaystyle \sum_{n=1}^\infty $
\quad
$\displaystyle \sum_{n=1}^\infty $
\quad

\vfill
